src/ModSimStutter.v
@@ -505,24 +505,24 @@ Module ModSim.
     Variable md_src: Mod.t.
     Variable md_tgt: Mod.t.
 
-    Record mod_sim: Prop :=
-      mk {
-          wf: WF;
-          world: Type;
-          world_le: world -> world -> Prop;
-          I: (@shared md_src.(Mod.state) md_tgt.(Mod.state) md_src.(Mod.ident) md_tgt.(Mod.ident) wf nat_wf world) -> Prop;
+    (* Record mod_sim: Prop := *)
+    (*   mk { *)
+    (*       wf: WF; *)
+    (*       world: Type; *)
+    (*       world_le: world -> world -> Prop; *)
+    (*       I: (@shared md_src.(Mod.state) md_tgt.(Mod.state) md_src.(Mod.ident) md_tgt.(Mod.ident) wf nat_wf world) -> Prop; *)
 
-          init_thread_id: TIdSet.t;
-          (* INV should hold for all current existing thread_id *)
-          init: forall im_tgt, exists im_src w,
-            I (init_thread_id, im_src, im_tgt, md_src.(Mod.st_init), md_tgt.(Mod.st_init), w);
+    (*       init_thread_id: TIdSet.t; *)
+    (*       (* INV should hold for all current existing thread_id *) *)
+    (*       init: forall im_tgt, exists im_src w, *)
+    (*         I (init_thread_id, im_src, im_tgt, md_src.(Mod.st_init), md_tgt.(Mod.st_init), w); *)
 
-          (* init_thread_id: TIdSet.t; *)
-          (* init: forall im_tgt, exists im_src w, *)
-          (*   I (init_thread_id, init_thread_id, im_src, im_tgt, md_src.(Mod.st_init), md_tgt.(Mod.st_init), w); *)
+    (*       (* init_thread_id: TIdSet.t; *) *)
+    (*       (* init: forall im_tgt, exists im_src w, *) *)
+    (*       (*   I (init_thread_id, init_thread_id, im_src, im_tgt, md_src.(Mod.st_init), md_tgt.(Mod.st_init), w); *) *)
 
-          funs: forall fn args, local_sim world_le I (@eq Val) (md_src.(Mod.funs) fn args) (md_tgt.(Mod.funs) fn args);
-        }.
+    (*       funs: forall fn args, local_sim world_le I (@eq Val) (md_src.(Mod.funs) fn args) (md_tgt.(Mod.funs) fn args); *)
+    (*     }. *)
 
     (* Record local_sim: Prop := *)
     (*   mk { *)
